factor out pointwise equality SVT

theories/diffpriv/examples/sparse_vector_technique.v
@@ -35,17 +35,7 @@ Section svt.
   Qed.
 
 
-  (* above_threshold ((num/den) : Q) (T : Z) (db : DB) (qᵢ : DB -o Z) : option (DB -o Z)  *)
-  (* "give me ↯ε and I'll privately find a query qᵢ above T" *)
-
-  (* in terms of affine / quantitative resources: *)
-  (* "give me ↯ε and I'll privately find a query qᵢ above T ONCE" *)
-  (* "for ↯ε you get a value that you can use once to privately find a query qᵢ above T" *)
-
-
-  (* { ↯ ε } A_T T { f . f : (DB -o Z) -> DB -o option Z }  *)
-
-  (* We can give the following naive specs: *)
+  (* We can give the following specs: *)
   (* { ↯ ε } A_T T ~ AT T
      { f f' . AUTH
             ∗ ∀ db db' : adjacent, ∀ q : 1-sensitive,
@@ -54,7 +44,11 @@ Section svt.
 [or pointwise eq:]
               ∀ R , { AUTH } f db qi ~ f db' qi { b b' : bool . ⌜b = R -> b' = R⌝ ∗ (⌜R = false⌝ -∗ AUTH) }
      }  *)
-  Definition above_threshold : val :=
+
+  (* If we add a flag to track whether an above-threshold query has been found, we can remain
+  private (and return AUTH) even after finding such a query by returning None. Probably not very
+  useful in practice. *)
+  Definition above_threshold_reset : val :=
     λ:"num" "den" "T",
       let: "T'" := Laplace "num" (#2*"den") "T" in
       let: "reset" := ref #false in
@@ -73,120 +67,14 @@ Section svt.
         in "f".
 
   (* We don't actually need `reset` since it is always set to `false` so long as a client holds AUTH. *)
-  Definition above_threshold_no_flag : val :=
+  Definition above_threshold : val :=
     λ:"num" "den" "T",
       let: "T'" := Laplace "num" (#2*"den") "T" in
       λ:"db" "qi",
         let: "vi" := Laplace "num" (#4*"den") ("qi" "db") in
         "T'" ≤ "vi".
 
-
-  (* For the version with the flag, we can prove the following point-wise spec where the
-  postcondition does some additional book-keeping to connect the result R to the return values when
-  we decide on whether AUTH should be returned. *)
-  Lemma above_threshold_online_spec_pw (num den T : Z) (εpos : 0 < IZR num / IZR den) `(dDB : Distance DB) (db db' : DB) (adj : dDB db db' <= 1) K :
-    ↯m (IZR num / IZR den) -∗
-    ⤇ fill K ((Val above_threshold) #num #den #T (Val (inject db')))
-    -∗
-    WP (Val above_threshold) #num #den #T (Val (inject db))
-       {{ f, ∃ f' : val,
-             ⤇ fill K (Val f') ∗
-             ∃ AUTH : iProp Σ,
-               AUTH ∗
-               ( ∀ q, wp_sensitive (Val q) 1 dDB dZ -∗
-                      AUTH -∗
-                      ⤇ fill K (f' q) -∗
-                      ∀ R : bool,
-                        WP (Val f) (Val q)
-                          {{ v, ∃ v', ⤇ fill K (Val v') ∗
-                                      ⌜ v = SOMEV #R → v' = SOMEV #R ⌝ ∗
-                                      (⌜R = false ∧ v = v' ∧ v = SOMEV #R⌝ -∗ AUTH)
-               }} )
-       }}.
-  Proof with (tp_pures ; wp_pures).
-    iIntros "ε rhs". rewrite /above_threshold...
-    tp_bind (Laplace _ _ _). wp_bind (Laplace _ _ _).
-    set (ε := (IZR num / IZR den)). replace ε with (ε / 2 + ε / 2) by real_solver.
-    fold ε in εpos.
-    iDestruct (ecm_split with "ε") as "[ε ε']". 1,2: real_solver.
-    iApply (hoare_couple_laplace _ _ 1%Z 1%Z with "[$rhs ε']") => //.
-    1: apply Zabs_ind ; lia.
-    1: rewrite mult_IZR ; apply Rdiv_pos_pos. 1,2: real_solver.
-    { iApply ecm_eq. 2: iFrame. subst ε. replace (IZR (2 * den)) with (2 * IZR den).
-      2: qify_r ; zify_q ; lia.
-      field. eapply Rdiv_pos_den_0 => //.
-    }
-    iIntros (T') "!> rhs" => /=...
-    tp_alloc as reset_r "reset_r". wp_alloc reset_l as "reset_l"...
-    iModIntro. iExists _. iFrame.
-    iExists (↯m (ε / 2) ∗ reset_r ↦ₛ #false ∗ reset_l ↦ #false)%I. iFrame.
-    iIntros "%q q_sens (ε & reset_r & reset_l) rhs %R"... tp_load. wp_load...
-
-    tp_bind (q _). wp_bind (q _). rewrite /wp_sensitive.
-    iSpecialize ("q_sens" $! _ _ db db'). iSpecialize ("q_sens" with "rhs").
-    Unshelve. 2: lra.
-    iPoseProof (wp_frame_l with "[reset_r $q_sens]") as "q_sens". 1: iAssumption.
-    iPoseProof (wp_frame_l with "[reset_l $q_sens]") as "q_sens". 1: iAssumption.
-    iPoseProof (wp_frame_l with "[ε $q_sens]") as "q_sens". 1: iAssumption.
-    iApply (wp_mono with "q_sens").
-    iIntros (?) "(ε & reset_l & reset_r & %vq_l & %vq_r & -> & rhs & %adj')" => /=...
-    assert (-1 <= vq_l - vq_r <= 1)%Z as [].
-    {
-      rewrite Rmult_1_l in adj'.
-      assert (dZ vq_l vq_r <= 1) as h by (etrans ; eauto).
-      revert h.
-      rewrite /dZ/distance Rabs_Zabs.
-      apply Zabs_ind ; intros ? h; split.
-      all: pose proof (le_IZR _ _ h) ; lia.
-    }
-    (* case on whether the result is the one that will get released (pweq) *)
-    destruct R eqn:HR.
-    - tp_bind (Laplace _ _ _). wp_bind (Laplace _ _ _).
-      iApply (hoare_couple_laplace vq_l vq_r 1%Z 2%Z with "[$rhs ε]") => //.
-      1: apply Zabs_ind ; lia.
-      1: rewrite mult_IZR ; apply Rdiv_pos_pos ; real_solver.
-      { subst ε. iApply ecm_eq. 2: iFrame. rewrite mult_IZR. field. eapply Rdiv_pos_den_0 => //. }
-      iIntros "%vi !> rhs" => /=...
-      case_bool_decide (_ (T' + 1)%Z _) ; tp_pures ; try tp_store ; tp_pures. all: case_bool_decide...
-      all: try tp_store ; try wp_store ; try tp_pures ; try wp_pures.
-      + iFrame. iModIntro. iSplitR. 1: done.
-        iIntros ((h_R & h_vv' & h_vR)). exfalso. inversion h_R.
-      + exfalso. lia.
-      + exfalso. lia.
-      + iFrame. iSplitR. 1: done. iModIntro.
-        iIntros ((h_R & h_vv' & h_vR)). exfalso. inversion h_R.
-    - tp_bind (Laplace _ _ _). wp_bind (Laplace _ _ _).
-      iMod ecm_zero as "ε0".
-      iApply (hoare_couple_laplace vq_l vq_r (vq_r - vq_l)%Z 0%Z with "[$rhs ε0]") => //.
-      1: apply Zabs_ind ; lia.
-      1: rewrite mult_IZR ; apply Rdiv_pos_pos ; real_solver.
-      1: rewrite Rmult_0_l ; iFrame.
-      iIntros "%vi !> rhs" => /=...
-      case_bool_decide (_ (T' + 1)%Z _) ; tp_pures ; try tp_store ; tp_pures. all: case_bool_decide...
-      all: try tp_store ; try wp_store ; try tp_pures ; try wp_pures.
-      + iFrame. iModIntro. iSplitR. 1: done.
-        iIntros ((_h_R & h_vv' & h_vR)). exfalso. inversion h_vR.
-      + exfalso. lia.
-      + iFrame. iModIntro. iSplitR. 1: done.
-        iIntros ((_h_R & h_vv' & h_vR)). exfalso. inversion h_vR.
-      + iFrame. done.
-  Qed.
-
   (* The spec that AT satisfies after initialising T'. *)
-  Definition AT_spec_pw (AUTH : iProp Σ) (f f' : val) : iProp Σ :=
-    □ ∀ (DB : Type) (dDB : Distance DB) (db db' : DB)
-      (_ : dDB db db' <= 1) (q : val) (K0 : list ectx_item),
-      wp_sensitive q 1 dDB dZ -∗
-      AUTH -∗
-      ⤇ fill K0 (f' (inject db') q) -∗
-      ∀ R : bool,
-        WP f (inject db) q
-          {{ v,
-               ∃ v' : val, ⤇ fill K0 v' ∗ ⌜v = #R → v' = #R⌝ ∗
-                           ∃ (b b' : bool), ⌜v = #b⌝ ∗ ⌜v' = #b'⌝ ∗
-                           (⌜R = false⌝ -∗ AUTH) }}
-  .
-
   Definition AT_spec (AUTH : iProp Σ) (f f' : val) : iProp Σ :=
     □ ∀ (DB : Type) (dDB : Distance DB) (db db' : DB)
       (_ : dDB db db' <= 1) (q : val) (K0 : list ectx_item),
@@ -197,216 +85,14 @@ Section svt.
         {{ v,
              ∃ v' : val, ⤇ fill K0 v' ∗ ⌜v = v'⌝ ∗
                            ∃ (b b' : bool), ⌜v = #b⌝ ∗ ⌜v' = #b'⌝ ∗
-                           (⌜b = false⌝ -∗ AUTH) }}
-  .
-
-
-  (* Removing ownership of the references from AUTH actually makes the postcondition simpler.
-     This is basically the less-naive version of the point-wise equality spec. *)
-  Lemma above_threshold_online_no_flag_spec_pw (num den T : Z) (εpos : 0 < IZR num / IZR den) K :
-    ↯m (IZR num / IZR den) -∗
-    ⤇ fill K ((Val above_threshold_no_flag) #num #den #T)
-    -∗
-    WP (Val above_threshold_no_flag) #num #den #T
-       {{ f, ∃ f' : val,
-             ⤇ fill K (Val f') ∗
-             ∃ AUTH : iProp Σ,
-               AUTH ∗
-               AT_spec_pw AUTH f f'
-       }}.
-  Proof with (tp_pures ; wp_pures).
-    iIntros "ε rhs". rewrite /above_threshold_no_flag...
-    tp_bind (Laplace _ _ _). wp_bind (Laplace _ _ _).
-    set (ε := (IZR num / IZR den)). replace ε with (ε / 2 + ε / 2) by real_solver.
-    fold ε in εpos.
-    iDestruct (ecm_split with "ε") as "[ε ε']". 1,2: real_solver.
-    iApply (hoare_couple_laplace _ _ 1%Z 1%Z with "[$rhs ε']") => //.
-    1: apply Zabs_ind ; lia.
-    1: rewrite mult_IZR ; apply Rdiv_pos_pos. 1,2: real_solver.
-    { iApply ecm_eq. 2: iFrame. subst ε. replace (IZR (2 * den)) with (2 * IZR den).
-      2: qify_r ; zify_q ; lia.
-      field. eapply Rdiv_pos_den_0 => //. }
-    iIntros (T') "!> rhs" => /=...
-    iModIntro. iExists _. iFrame "rhs".
-    iExists (↯m (ε / 2))%I. iFrame "ε". clear K.
-    iModIntro.
-    iIntros (?????) "%q %K q_sens ε rhs %R"...
-
-    tp_bind (q _) ; wp_bind (q _). rewrite /wp_sensitive.
-    iSpecialize ("q_sens" $! _ _ db db'). iSpecialize ("q_sens" with "rhs").
-    Unshelve. 2: lra.
-
-    iApply (wp_strong_mono'' with "q_sens [ε]") => //.
-    iIntros (?) "(%vq_l & %vq_r & -> & rhs & %adj')" => /=...
-    assert (-1 <= vq_l - vq_r <= 1)%Z as [].
-    {
-      rewrite Rmult_1_l in adj'.
-      assert (dZ vq_l vq_r <= 1) as h by (etrans ; eauto).
-      revert h. rewrite /dZ/distance Rabs_Zabs.
-      apply Zabs_ind ; intros ? h; split.
-      all: pose proof (le_IZR _ _ h) ; lia.
-    }
-    tp_bind (Laplace _ _ _). wp_bind (Laplace _ _ _).
-    (* case on whether the result is the one that will get released (pweq) *)
-    destruct R eqn:HR.
-    - iApply (hoare_couple_laplace vq_l vq_r 1%Z 2%Z with "[$rhs ε]") => //.
-      1: apply Zabs_ind ; lia.
-      1: rewrite mult_IZR ; apply Rdiv_pos_pos ; real_solver.
-      { subst ε. iApply ecm_eq. 2: iFrame. rewrite mult_IZR. field. eapply Rdiv_pos_den_0 => //. }
-      iIntros "%z_l !> rhs" => /=. tp_pures.
-      case_bool_decide (_ (T' + 1)%Z _)...
-      all: destruct_decide (bool_decide_reflect (T' ≤ z_l)%Z) as res_l.
-      all: iFrame "rhs" ; iModIntro.
-      + iSplitR => //. iExists true,true. do 2 iSplitR => //. iIntros (h_R). exfalso. inversion h_R.
-      + exfalso. lia.
-      + exfalso. lia.
-      + iSplitR => //. iExists false, false. do 2 iSplitR => //. iIntros (h_R). exfalso. inversion h_R.
-    - iMod ecm_zero as "ε0".
-      iApply (hoare_couple_laplace vq_l vq_r (vq_r - vq_l)%Z 0%Z with "[$rhs ε0]") => //.
-      1: apply Zabs_ind ; lia.
-      1: rewrite mult_IZR ; apply Rdiv_pos_pos ; real_solver.
-      1: rewrite Rmult_0_l ; iFrame.
-      iIntros "%z_l !> rhs" => /=...
-      case_bool_decide (_ (T' + 1)%Z _).
-      all: destruct_decide (bool_decide_reflect (T' ≤ z_l)%Z) as res_l ; iModIntro ; iFrame "rhs".
-      all: iSplitR ; [|by (iExists _,_ ; iFrame "ε")].
-      + iIntros (Rf). inversion Rf.
-      + exfalso. lia.
-      + iIntros (Rf). inversion Rf.
-      + done.
-  Qed.
-
-  (* Clearly, getting the result of the comparison helps. How much does it help? *)
-  (* If we get R before having to pick the coupling for the noisy T', then we can just couple the first
-     Laplacian so that the comparisons are synchronised and use the error for the second Laplace instead. *)
-  (* Only half of the error has to be provided upfront, the other half is to be paid for a query
-     that produces an above-threshold result. *)
-  (* We can reformulate the postcondition ; no need to return AUTH since the error
-     was only provided in the case where it would have been consumed. *)
-  (* At first glance, this spec may seem silly. But for now, it is unclear if this spec is
-     substantially worse than the other pointwise-equality spec. If Above Threshold is simply run in
-     a loop until a good query is found, then we would presumably have to know the index of the good
-     query in advance in both cases; maybe that would suffice to conjure up `R` at the time of
-     initialization of AT. *)
-  Lemma above_threshold_online_no_flag_spec_pw_no_AUTH' (num den T : Z)
-    (εpos : 0 < IZR num / IZR den) K (R : bool) :
-    ↯m (IZR num / (2 * IZR den)) -∗
-    ⤇ fill K ((Val above_threshold_no_flag) #num #den #T)
-    -∗
-    WP (Val above_threshold_no_flag) #num #den #T
-       {{ f, ∃ f' : val,
-             ⤇ fill K (Val f') ∗
-               ( ∀ `(dDB : Distance DB) (db db' : DB) (adj : dDB db db' <= 1) q K,
-                   wp_sensitive (Val q) 1 dDB dZ -∗
-                      ⤇ fill K (f' (Val (inject db')) q) -∗
-                      (if R then ↯m (IZR num / (2 * IZR den)) else emp) -∗
-                        WP (Val f) (Val (inject db)) (Val q)
-                          {{ v, ∃ v', ⤇ fill K (Val v') ∗
-                                      ⌜ v = #R → v' = #R ⌝
-               }} )
-       }}.
-  Proof with (tp_pures ; wp_pures).
-    iIntros "ε rhs". rewrite /above_threshold_no_flag...
-    tp_bind (Laplace _ _ _). wp_bind (Laplace _ _ _).
-    set (ε := (IZR num / 2 * IZR den)).
-    fold ε in εpos.
-    (* case on whether the result is the one that will get released (pweq) *)
-    destruct R eqn:HR.
-    {
-      iApply (hoare_couple_laplace _ _ 1%Z 1%Z with "[$rhs ε]") => //.
-      1: apply Zabs_ind ; lia.
-      1: rewrite mult_IZR ; apply Rdiv_pos_pos ; real_solver.
-      { iApply ecm_eq. 2: iFrame. subst ε. replace (IZR (2 * den)) with (2 * IZR den).
-        2: qify_r ; zify_q ; lia.
-        field. eapply Rdiv_pos_den_0 => //. }
-      iIntros (T') "!> rhs" => /=...
-      iModIntro. iExists _. iFrame "rhs". clear K.
-      iIntros (?????) "%q %K q_sens rhs ε" => /=...
-
-      tp_bind (q _) ; wp_bind (q _). rewrite /wp_sensitive.
-      iSpecialize ("q_sens" $! _ _ db db'). iSpecialize ("q_sens" with "rhs").
-      Unshelve. 2: lra.
-
-      iApply (wp_strong_mono'' with "q_sens [ε]") => //.
-      iIntros (?) "(%vq_l & %vq_r & -> & rhs & %adj')" => /=...
-      assert (-1 <= vq_l - vq_r <= 1)%Z as [adj_lb adj_ub].
-      {
-        rewrite Rmult_1_l in adj'.
-        assert (dZ vq_l vq_r <= 1) as h by (etrans ; eauto).
-        revert h. rewrite /dZ/distance Rabs_Zabs.
-        apply Zabs_ind ; intros ? h; split.
-        all: pose proof (le_IZR _ _ h) ; lia.
-      }
-      tp_bind (Laplace _ _ _). wp_bind (Laplace _ _ _).
-      iApply (hoare_couple_laplace vq_l vq_r 1%Z 2%Z with "[$rhs ε]") => //.
-      1: apply Zabs_ind ; lia.
-      1: rewrite mult_IZR ; apply Rdiv_pos_pos ; real_solver.
-      { subst ε. iApply ecm_eq. 2: iFrame. rewrite mult_IZR. field. eapply Rdiv_pos_den_0 => //. }
-      iIntros "%z_l !> rhs" => /=. tp_pures.
-      case_bool_decide (_ (T' + 1)%Z _) as res_r...
-      all: destruct_decide (bool_decide_reflect (T' ≤ z_l)%Z) as res_l.
-      all: iFrame "rhs" ; iModIntro.
-      + done.
-      + exfalso. lia.
-      + exfalso. lia.
-      + done.
-    }
-
-    {
-      iMod ecm_zero as "ε0".
-      iApply (hoare_couple_laplace _ _ 0%Z 0%Z with "[$rhs ε0]") => //.
-      1: apply Zabs_ind ; lia.
-      1: rewrite mult_IZR ; apply Rdiv_pos_pos ; real_solver.
-      { iApply ecm_eq. 2: iFrame. lra. }
-      iIntros (T') "!> rhs" => /=...
-      iModIntro. iExists _. iFrame "rhs". clear K.
-      iIntros (?????) "%q %K q_sens rhs ε'" => /=...
-
-      tp_bind (q _) ; wp_bind (q _). rewrite /wp_sensitive.
-      iSpecialize ("q_sens" $! _ _ db db'). iSpecialize ("q_sens" with "rhs").
-      Unshelve. 2: lra.
-
-      iApply (wp_strong_mono'' with "q_sens [ε]") => //.
-      iIntros (?) "(%vq_l & %vq_r & -> & rhs & %adj')" => /=...
-      assert (-1 <= vq_l - vq_r <= 1)%Z as [adj_lb adj_ub].
-      {
-        rewrite Rmult_1_l in adj'.
-        assert (dZ vq_l vq_r <= 1) as h by (etrans ; eauto).
-        revert h. rewrite /dZ/distance Rabs_Zabs.
-        apply Zabs_ind ; intros ? h; split.
-        all: pose proof (le_IZR _ _ h) ; lia.
-      }
-      tp_bind (Laplace _ _ _). wp_bind (Laplace _ _ _).
-      iApply (hoare_couple_laplace vq_l vq_r 0%Z 1%Z with "[$rhs ε]") => //.
-      1: apply Zabs_ind ; lia.
-      1: rewrite mult_IZR ; apply Rdiv_pos_pos ; real_solver.
-      1: rewrite Rmult_1_l mult_IZR.
-      (* Actually, only half the error we have is needed. *)
-      { subst ε. iApply ecm_weaken. 2: iFrame. split.
-        - apply Rdiv_nneg_nneg ; lra.
-        - rewrite (Rmult_comm 4). rewrite (Rmult_comm 2).
-          rewrite Rdiv_mult_distr. rewrite Rdiv_mult_distr.
-          rewrite /Rdiv. apply Rmult_le_compat_l.
-          1: lra. lra.
-      }
-      iIntros "%z_l !> rhs" => /=...
-      case_bool_decide (_ (T' + 0)%Z _) as res_r.
-      all: rewrite !Zplus_0_r in res_r.
-      all: destruct_decide (bool_decide_reflect (T' ≤ z_l)%Z) as res_l ; iModIntro ; iFrame "rhs".
-      + done.
-      + exfalso. clear -res_l res_r. done.
-      + exfalso. clear -res_l res_r. done.
-      + done.
-    }
-  Qed.
-
-
+                           (⌜b = false⌝ -∗ AUTH) }}.
 
   (* SVT calibrates the noise by simply dividing up the initial budget ε =
   num/den over the number of queries c exceeding the threshold T and running
   each "above_threshold" query with privacy budget ε/c. *)
   (* SVT : ℚ → ℤ → ℕ → DB → (DB → Z) → option 𝔹 *)
-  Definition SVT_online (num den : Z) : val :=
+  (* This definition is unused; instead we construct SVT as a client of AT. *)
+  Definition SVT_online_AT_inlined (num den : Z) : val :=
     λ:"T" "c",
       let: "found_above_T" := ref #true in
       let: "T'" := ref "T" in
@@ -427,67 +113,37 @@ Section svt.
                  #false)
       in "f".
 
-  (* SVT expressed in terms of Above Threshold, for modular analysis. *)
-  (* NB: This is different from bounded oracles ("q_calls" in Approxis) because
-     we only count calls to above_threshold that return a #true result. *)
-  Definition SVT_AT_online (num den : Z) : val :=
-    λ:"T" "c",
-      let: "count" := ref #0 in
-      let: "AT" := ref (above_threshold #num ("c" * #den) "T" "db") in
-      λ:"db" "qi",
-        if: "c" < !"count" then NONE else
-          match: !"AT" "db" "qi" with
-          | SOME "v" =>
-              (if: "v" then
-                 ("AT" <- (above_threshold #num ("c" * #den) "T" "db") ;;
-                  "count" <- !"count" + #1)
-               else #()) ;;
-              SOME "v"
-          | NONE => NONE (* should never happen because we always reset AT diligently *)
-          end.
+  (* SVT expressed in terms of Above Threshold, for modular analysis.
 
+     The reference "AT" stores an initialised above_threshold at all times. We need to keep track
+     of the number of `true` results we returned in the reference "count" because we can only
+     perform N initialisations of AT. *)
+  (* NB: This is different from bounded oracles ("q_calls" in Approxis) because we only count calls
+     to above_threshold that return a #true result: we invoke the closure not only N many times,
+     but until we a `true` result N times. *)
 
-  (* SVT without counting, expressed in terms of Above Threshold without Flag, for modular analysis. *)
-  Definition SVT_AT_NF_NC_online : val :=
-    λ:"num" "den" "T" "N",
-      let: "AT" := ref (above_threshold_no_flag "num" "den" "T") in
-      λ:"db" "qi",
-        let: "bq" := !"AT" "db" "qi" in
-        (if: "bq" then
-           "AT" <- (above_threshold_no_flag "num" "den" "T")
-         else #()) ;;
-        "bq"
-  .
-
-  (* SVT with counting but w/o flag *)
-  Definition SVT_AT_NF_online : val :=
+  Definition oSVT : val :=
     λ:"num" "den" "T" "N",
       let: "count" := ref ("N" - #1) in
-      let: "AT" := ref (above_threshold_no_flag "num" "den" "T") in
+      let: "AT" := ref (above_threshold "num" "den" "T") in
       λ:"db" "qi",
         let: "bq" := !"AT" "db" "qi" in
         (if: #0 < !"count" `and` "bq" then
-           ("AT" <- (above_threshold_no_flag "num" "den" "T") ;;
+           ("AT" <- (above_threshold "num" "den" "T") ;;
             "count" <- !"count" - #1)
          else #()) ;;
         "bq".
 
 
-  (* Hypothetically, if we didn't work with pointwise equalities, would things get easier? *)
-  (* Let's prove the non-pw spec for AT from hoare_couple_laplace_choice. *)
-  Lemma above_threshold_online_no_flag_spec (num den T : Z) (εpos : 0 < IZR num / IZR den) K :
+  (* We prove the (non-pw) spec for oAT from hoare_couple_laplace_choice. *)
+  Lemma above_threshold_online_AT_spec (num den T : Z) (εpos : 0 < IZR num / IZR den) K :
     ↯m (IZR num / IZR den) -∗
-    ⤇ fill K ((Val above_threshold_no_flag) #num #den #T)
-    -∗
-    WP (Val above_threshold_no_flag) #num #den #T
-       {{ f, ∃ f' : val,
-             ⤇ fill K (Val f') ∗
-             ∃ AUTH : iProp Σ,
-               AUTH ∗
-               AT_spec AUTH f f'
-       }}.
+    ⤇ fill K ((Val above_threshold) #num #den #T)
+    -∗ WP (Val above_threshold) #num #den #T
+         {{ f, ∃ (f' : val) (AUTH : iProp Σ),
+               ⤇ fill K (Val f') ∗ AUTH ∗ AT_spec AUTH f f' }}.
   Proof with (tp_pures ; wp_pures).
-    iIntros "ε rhs". rewrite /above_threshold_no_flag...
+    iIntros "ε rhs". rewrite /above_threshold...
     tp_bind (Laplace _ _ _). wp_bind (Laplace _ _ _).
     set (ε := (IZR num / IZR den)). replace ε with (ε / 2 + ε / 2) by real_solver.
     fold ε in εpos.
@@ -501,13 +157,10 @@ Section svt.
     iIntros (T') "!> rhs" => /=...
     iModIntro. iExists _. iFrame "rhs".
     iExists (↯m (ε / 2))%I. iFrame "ε". clear K.
-    iModIntro.
-    iIntros (?????) "%q %K q_sens ε rhs"...
-
+    iModIntro. iIntros (?????) "%q %K q_sens ε rhs"...
     tp_bind (q _) ; wp_bind (q _). rewrite /wp_sensitive.
     iSpecialize ("q_sens" $! _ _ db db'). iSpecialize ("q_sens" with "rhs").
     Unshelve. 2: lra.
-
     iApply (wp_strong_mono'' with "q_sens [ε]") => //.
     iIntros (?) "(%vq_l & %vq_r & -> & rhs & %adj')" => /=...
     assert (-1 <= vq_l - vq_r <= 1)%Z as [].
@@ -518,13 +171,13 @@ Section svt.
       apply Zabs_ind ; intros ? h; split.
       all: pose proof (le_IZR _ _ h) ; lia.
     }
-  tp_bind (Laplace _ _ _). wp_bind (Laplace _ _ _).
-  iApply (hoare_couple_laplace_choice vq_l (vq_r) T' with "[$]") => //.
-  1: apply Zabs_ind ; lia.
-  1: rewrite mult_IZR ; apply Rdiv_pos_pos. 1,2: real_solver.
-  { subst ε. rewrite mult_IZR. field. eapply Rdiv_pos_den_0 => //. }
-  iIntros "%z !> (%z' & rhs & hh)".
-  iDestruct "hh" as "[%h_above | [%h_below ε]]".
+    tp_bind (Laplace _ _ _). wp_bind (Laplace _ _ _).
+    iApply (hoare_couple_laplace_choice vq_l (vq_r) T' with "[$]") => //.
+    1: apply Zabs_ind ; lia.
+    1: rewrite mult_IZR ; apply Rdiv_pos_pos. 1,2: real_solver.
+    { subst ε. rewrite mult_IZR. field. eapply Rdiv_pos_den_0 => //. }
+    iIntros "%z !> (%z' & rhs & hh)".
+    iDestruct "hh" as "[%h_above | [%h_below ε]]".
     - simpl... case_bool_decide.
       + iFrame. iModIntro. case_bool_decide. 2: lia. iSplit => //.
         iExists true,true. repeat iSplitR => //. iIntros (?). done.
@@ -537,12 +190,12 @@ Section svt.
 
 
   (* We can now prove the non-pw spec for oSVT without much pain. *)
-  Lemma SVT_online_diffpriv_notpw (num den T : Z) (N : nat) (Npos : (0 < N)%nat) K :
+  Lemma SVT_online_diffpriv (num den T : Z) (N : nat) (Npos : (0 < N)%nat) K :
     let ε := IZR num / IZR den in
     ∀ (εpos : 0 < ε),
       ↯m (N * ε) -∗
-      ⤇ fill K (SVT_AT_NF_online #num #den #T #N) -∗
-      WP SVT_AT_NF_online #num #den #T #N
+      ⤇ fill K (oSVT #num #den #T #N) -∗
+      WP oSVT #num #den #T #N
         {{ f, ∃ (f' : val) (iSVT : nat → iProp Σ),
               ⤇ fill K f' ∗
               iSVT N ∗
@@ -550,26 +203,26 @@ Section svt.
                   wp_sensitive (Val q) 1 dDB dZ -∗
                   ⤇ fill K (Val f' (inject db') q) -∗
                   ∀ n, iSVT (S n) -∗
-                       WP Val f (inject db) q {{v, ∃ v' : val,
-                               ⤇ fill K (Val v') ∗
-                               ⌜v = v'⌝ ∗ ∃ RES : bool, ⌜v = #RES⌝ ∗ iSVT (if RES then n else S n) }}
+                       WP Val f (inject db) q
+                         {{v, ⤇ fill K (Val v) ∗
+                              ∃ b : bool, ⌜v = #b⌝ ∗ iSVT (if b then n else S n) }}
         )}}.
   Proof with (tp_pures ; wp_pures).
     (* make sure we have at least enough credit to initialise AT once *)
     destruct N as [|N'] ; [lia|] ; clear Npos.
-    iIntros (??) "SNε rhs". rewrite /SVT_AT_NF_online...
+    iIntros (??) "SNε rhs". rewrite /oSVT...
     tp_alloc as count_r "count_r". wp_alloc count_l as "count_l"...
-    tp_bind (above_threshold_no_flag _ _ _) ; wp_bind (above_threshold_no_flag _ _ _).
+    tp_bind (above_threshold _ _ _) ; wp_bind (above_threshold _ _ _).
     assert (INR (N'+1)%nat ≠ 0). { replace 0 with (INR 0) => //. intros ?%INR_eq. lia. }
     replace (S N' * ε) with (ε + N' * ε).
     2:{ replace (S N') with (N'+1)%nat by lia. replace (INR (N'+1)) with (N' + 1) by real_solver. lra. }
     iDestruct (ecm_split with "SNε") as "[ε Nε]". 1,2: real_solver.
-    opose proof (above_threshold_online_no_flag_spec num den T _) as AT.
+    opose proof (above_threshold_online_AT_spec num den T _) as AT.
     1: done.
     iPoseProof (AT with "[ε] [rhs]") as "AT" => // ; clear AT.
     iApply (wp_strong_mono'' with "AT").
     replace (S N') with (N'+1)%nat by lia.
-    iIntros "%f (%f' & rhs & %AUTH & auth & AT) /=".
+    iIntros "%f (%f' & %AUTH & rhs & auth & AT) /=".
     tp_alloc as ref_f' "ref_f'". wp_alloc ref_f as "ref_f"...
     iModIntro. iExists _. iFrame "rhs".
     set (iSVT := (λ n : nat,
@@ -598,250 +251,37 @@ Section svt.
     - tp_load ; wp_load...
       rewrite /= !Nat.sub_0_r.
       destruct n as [|n']...
-      { rewrite /iSVT. iExists _. simpl. iFrame.
-        iSplitR. 1: done. iExists bq'. subst. simpl. done. }
+      { rewrite /iSVT. iFrame. iExists _. iSplitR. 1: done. simpl. done. }
       replace (S n' * ε) with (ε + n' * ε).
       2:{ replace (S n') with (n'+1)%nat by lia. replace (INR (n'+1)) with (n' + 1) by real_solver. lra. }
       iDestruct (ecm_split with "nε") as "[ε n'ε]". 1,2: real_solver.
       simpl. simplify_eq...
-      tp_bind (above_threshold_no_flag _ _ _) ; wp_bind (above_threshold_no_flag _ _ _).
-      opose proof (above_threshold_online_no_flag_spec num den T _) as AT_pw.
+      tp_bind (above_threshold _ _ _) ; wp_bind (above_threshold _ _ _).
+      opose proof (above_threshold_online_AT_spec num den T _) as AT_pw.
       1: done.
       iPoseProof (AT_pw with "[ε] [rhs]") as "AT_pw" => // ; clear AT_pw.
       iApply (wp_strong_mono'' with "AT_pw [-]").
-      iIntros "%g (%g' & rhs & %AUTH' & auth & AT') /=".
+      iIntros "%g (%g' & %AUTH' & rhs & auth & AT') /=".
       tp_store ; wp_store... tp_load... tp_store ; wp_load... wp_store.
-      iFrame. iSplitR. 1: done.
-      iExists true. iSplitR. 1: done. rewrite /iSVT. simpl.
+      iFrame. iExists true. iSplitR. 1: done.
+      rewrite /iSVT. simpl.
       replace ((n' - 0)%nat) with n' by lia. iFrame.
       replace (Z.of_nat (S n') - 1)%Z with (Z.of_nat n') by lia. iFrame. done.
     - simpl... rewrite /= !Nat.sub_0_r. simplify_eq.
       iSpecialize ("maybe_auth" $! eq_refl).
       tp_load ; wp_load...
       destruct n as [|n']...
-      { rewrite /iSVT. iFrame. iSplitR. 1: done.
+      { rewrite /iSVT. iFrame.
         iExists false. iSplitR => //. simpl. iFrame.
         iExists TOKEN. iFrame. done.
       }
-      iFrame. iSplitR => //. iExists _ ; iSplitR => //. iSimpl. iFrame. iExists TOKEN. iFrame. done.
+      iFrame. iExists _ ; iSplitR => //. iSimpl. iFrame. iExists TOKEN. iFrame. done.
   Qed.
-
-  (* TODO move *)
-  Lemma AT_NF_safe num den T :
-    ⊢ WP (above_threshold_no_flag #num #den #T) {{ v, ⌜True⌝ }}.
-  Proof.
-    rewrite /above_threshold_no_flag.
-  Admitted.
-
-  (* TODO move *)
-  (* Pointwise equality spec for oSVT based on pweq oAT. *)
-  (* Crucially, the whole post-condition is guarded by ⌜v = #RES⌝. This is analogous to the
-     point-wise equality postcondition: only if the "guess" of RES was correct do we guarantee
-     anything about the RHS return value (v' = #RES) and the predicate iSVT. *)
-  Lemma SVT_online_diffpriv (num den T : Z) (N : nat) (Npos : (0 < N)%nat) K :
-    let ε := IZR num / IZR den in
-    ∀ (εpos : 0 < ε),
-      ↯m (N * ε) -∗
-      ⤇ fill K (SVT_AT_NF_online #num #den #T #N) -∗
-      WP SVT_AT_NF_online #num #den #T #N
-        {{ f, ∃ (f' : val) (iSVT : nat → iProp Σ),
-              ⤇ fill K f' ∗
-              iSVT N ∗
-              (∀ `(dDB : Distance DB) (db db' : DB) (adj : dDB db db' <= 1) (q : val) K,
-                  wp_sensitive (Val q) 1 dDB dZ -∗
-                  ⤇ fill K (Val f' (inject db') q) -∗
-                  ∀ n, iSVT (S n) -∗
-                       ∀ (RES : bool),
-                         WP Val f (inject db) q {{v, ∃ v' : val,
-                                 ⌜v = #RES⌝ -∗
-                                 (⤇ fill K (Val v') ∗ ⌜v' = #RES⌝ ∗ iSVT (if RES then n else S n)) }}
-        )}}.
-  Proof with (tp_pures ; wp_pures).
-    (* make sure we have at least enough credit to initialise AT once *)
-    destruct N as [|N'] ; [lia|] ; clear Npos.
-    iIntros (??) "SNε rhs". rewrite /SVT_AT_NF_online...
-    tp_alloc as count_r "count_r". wp_alloc count_l as "count_l"...
-    tp_bind (above_threshold_no_flag _ _ _) ; wp_bind (above_threshold_no_flag _ _ _).
-    assert (INR (N'+1)%nat ≠ 0). { replace 0 with (INR 0) => //. intros ?%INR_eq. lia. }
-    replace (S N' * ε) with (ε + N' * ε).
-    2:{ replace (S N') with (N'+1)%nat by lia. replace (INR (N'+1)) with (N' + 1) by real_solver. lra. }
-    iDestruct (ecm_split with "SNε") as "[ε Nε]". 1,2: real_solver.
-    opose proof (above_threshold_online_no_flag_spec_pw num den T _) as AT_pw.
-    1: done.
-    iPoseProof (AT_pw with "[ε] [rhs]") as "AT_pw" => // ; clear AT_pw.
-    iApply (wp_strong_mono'' with "AT_pw").
-    replace (S N') with (N'+1)%nat by lia.
-    iIntros "%f (%f' & rhs & %AUTH & auth & AT) /=".
-    tp_alloc as ref_f' "ref_f'". wp_alloc ref_f as "ref_f"...
-    iModIntro. iExists _. iFrame "rhs".
-    set (iSVT := (λ n : nat,
-                       if Nat.ltb 0%nat n then
-                         let n' := (n-1)%nat in
-                         count_l ↦ #n' ∗ count_r ↦ₛ #n' ∗
-                         ↯m (n' * ε) ∗ ∃ token f f',
-                           token ∗ ref_f ↦ f ∗ ref_f' ↦ₛ f' ∗ AT_spec_pw token f f'
-                       else emp
-                 )%I). iExists iSVT.
-    iSplitL.
-    { rewrite /iSVT /=. destruct (0 <? N'+1)%nat => //.
-      replace ((N'+1)%nat-1)%Z with (Z.of_nat N') by lia.
-      replace (N'+1-1)%nat with N' by lia. iFrame. }
-    clear f f'.
-    iIntros (???????) "q_sens rhs %n (count_l & count_r & nε & (%TOKEN & %f & %f' & auth & ref_f & ref_f' & #AT)) %RES"...
-    iCombine "AT" as "AT_cpy".
-    (* replace (S n - 1)%nat with n by lia. *)
-    tp_load ; wp_load. tp_bind (f' _ _) ; wp_bind (f _ _).
-    iSpecialize ("AT" $! _ _ _ _ adj _ _).
-    iSpecialize ("AT" with "q_sens auth rhs").
-    iSpecialize ("AT" $! RES).
-    iApply (wp_strong_mono'' with "AT").
-    iIntros "%vq (%vq' & rhs & %pweq & %bq & %bq' & -> & -> & maybe_auth)".
-    iSimpl in "rhs"...
-    destruct bq eqn:case_bq, RES eqn:case_RES.
-    - rewrite pweq //...
-      tp_load ; wp_load...
-      rewrite /= !Nat.sub_0_r.
-      destruct n as [|n']...
-      { rewrite /iSVT. simpl. iExists #true. iModIntro. iIntros. iFrame. done. }
-      replace (S n' * ε) with (ε + n' * ε).
-      2:{ replace (S n') with (n'+1)%nat by lia. replace (INR (n'+1)) with (n' + 1) by real_solver. lra. }
-      iDestruct (ecm_split with "nε") as "[ε n'ε]". 1,2: real_solver.
-      tp_bind (above_threshold_no_flag _ _ _) ; wp_bind (above_threshold_no_flag _ _ _).
-      opose proof (above_threshold_online_no_flag_spec_pw num den T _) as AT_pw.
-      1: done.
-      iPoseProof (AT_pw with "[ε] [rhs]") as "AT_pw" => // ; clear AT_pw.
-      iApply (wp_strong_mono'' with "AT_pw [-]").
-      iIntros "%g (%g' & rhs & %AUTH' & auth & AT') /=".
-      tp_store ; wp_store... tp_load... tp_store ; wp_load... wp_store.
-      iFrame. iModIntro. iIntros. iSplitR. 1: done.
-      rewrite /iSVT.
-      replace (Z.of_nat (S n' - 1)%nat) with (S n' - 1)%Z by lia. iFrame.
-      replace (S n' - 1)%nat with n' by lia. iFrame.
-    - simpl... rewrite /= !Nat.sub_0_r.
-      iSpecialize ("maybe_auth" $! eq_refl).
-      tp_load ; wp_load...
-      destruct n as [|n']...
-      { rewrite /iSVT. iFrame. iModIntro. iIntros (h). inversion h. }
-      wp_bind (above_threshold_no_flag _ _ _).
-
-  (*     iApply (wp_strong_mono'' with "AT_NF_safe"). iIntros...
-         wp_store ; wp_load ; wp_store. iExists _. iIntros "!>**". exfalso. done.
-       - simpl... rewrite /= !Nat.sub_0_r. tp_load ; wp_load...
-         destruct n as [|n']...
-         { rewrite /iSVT. iFrame. iModIntro. iIntros (h). inversion h. }
-         iExists _. iIntros "!>**". exfalso. done.
-       - rewrite pweq //... tp_load ; wp_load...
-         case_bool_decide...
-         +
-           iExists _. iIntros "!>**". iFrame. iSplitR. 1: done.
-           iExists TOKEN.
-           iSpecialize ("maybe_auth" $! eq_refl).
-           iFrame. done.
-         +
-           iExists _. iIntros "!>**". iFrame. iSplitR. 1: done.
-           iExists TOKEN.
-           iSpecialize ("maybe_auth" $! eq_refl).
-           iFrame. done.
-           Unshelve. all: easy.
-     Qed. *)
-  Abort.
-
-  Lemma SVT_online_diffpriv (num den T : Z) (N : nat) (Npos : (0 < N)%nat) K :
-    let ε := IZR num / IZR den in
-    ∀ (εpos : 0 < ε),
-      ↯m (N * ε) -∗
-      ⤇ fill K (SVT_AT_NF_NC_online #num #den #T #N) -∗
-      WP SVT_AT_NF_NC_online #num #den #T #N
-        {{ f, ∃ (f' : val) (iSVT : nat → iProp Σ),
-              ⤇ fill K f' ∗
-              iSVT N ∗
-              (∀ `(dDB : Distance DB) (db db' : DB) (adj : dDB db db' <= 1) (q : val) K,
-                  wp_sensitive (Val q) 1 dDB dZ -∗
-                  ⤇ fill K (Val f' (inject db') q) -∗
-                  ∀ n, iSVT (S n) -∗
-                       ∀ (RES : bool),
-                         WP Val f (inject db) q {{v, ∃ v' : val, ⌜v = #RES → v' = #RES⌝ ∗ iSVT (if RES then n else S n) }}
-        )}}.
-  Proof with (tp_pures ; wp_pures).
-    (* make sure we have at least enough credit to initialise AT once *)
-    destruct N as [|N'] ; [lia|] ; clear Npos.
-    iIntros (??) "SNε rhs". rewrite /SVT_AT_NF_NC_online...
-    tp_bind (above_threshold_no_flag _ _ _) ; wp_bind (above_threshold_no_flag _ _ _).
-    assert (INR (N'+1)%nat ≠ 0). { replace 0 with (INR 0) => //. intros ?%INR_eq. lia. }
-    replace (S N' * ε) with (ε + N' * ε).
-    2:{ replace (S N') with (N'+1)%nat by lia. replace (INR (N'+1)) with (N' + 1) by real_solver. lra. }
-    iDestruct (ecm_split with "SNε") as "[ε Nε]". 1,2: real_solver.
-    opose proof (above_threshold_online_no_flag_spec_pw num den T _) as AT_pw.
-    1: done.
-    iPoseProof (AT_pw with "[ε] [rhs]") as "AT_pw" => // ; clear AT_pw.
-    iApply (wp_strong_mono'' with "AT_pw").
-    replace (S N') with (N'+1)%nat by lia.
-    iIntros "%f (%f' & rhs & %AUTH & auth & AT) /=".
-    tp_alloc as ref_f' "ref_f'". wp_alloc ref_f as "ref_f"...
-    iModIntro. iExists _. iFrame "rhs".
-    set (iSVT := (λ n : nat,
-                       if Nat.ltb 0%nat n then
-                         ↯m ((n-1)%nat * ε) ∗ ∃ token f f',
-                           token ∗ ref_f ↦ f ∗ ref_f' ↦ₛ f' ∗ AT_spec_pw token f f'
-                       else emp
-                 )%I). iExists iSVT.
-    iSplitL.
-    { rewrite /iSVT /=. destruct (0 <? N'+1)%nat => //. replace (N'+1-1)%nat with N' by lia. iFrame. }
-    clear f f'.
-    iIntros (???????) "q_sens rhs %n (nε & (%TOKEN & %f & %f' & auth & ref_f & ref_f' & AT)) %RES"...
-    replace (S n - 1)%nat with n by lia.
-    tp_load ; wp_load. tp_bind (f' _ _) ; wp_bind (f _ _).
-    iSpecialize ("AT" $! _ _ _ _ adj _ _).
-    iSpecialize ("AT" with "q_sens auth rhs").
-    iSpecialize ("AT" $! RES).
-    iApply (wp_strong_mono'' with "AT").
-    iIntros "%vq (%vq' & rhs & %pweq & %bq & %bq' & -> & -> & maybe_auth)".
-    iSimpl in "rhs"...
-    iAssert (AT_spec_pw TOKEN f f') as "AT". 1: admit. (* should have been persistent *)
-    destruct bq eqn:case_bq, RES eqn:case_RES.
-    - rewrite pweq //...
-      (* We should only end up in this case if 0<n holds!
-         SVT shouldn't re-allocate another AT on the last (Nth) invocation since it won't get used.
-         Maybe it needs a counter?
-       *)
-      destruct (0 <? n)%nat eqn:n_pos => //.
-      2: admit.
-      iFrame.
-      tp_bind (above_threshold_no_flag _ _ _) ; wp_bind (above_threshold_no_flag _ _ _).
-      opose proof (above_threshold_online_no_flag_spec_pw num den T _) as AT_pw.
-      1: done.
-      iMod ecm_zero as "ε0".
-      iPoseProof (AT_pw with "[ε0] [rhs]") as "AT_pw" => // ; clear AT_pw.
-      1: admit.
-      iApply (wp_strong_mono'' with "AT_pw [-]").
-      iIntros "%g (%g' & rhs & %AUTH' & auth & AT') /=".
-      tp_store ; wp_store.
-      iFrame. iExists #true. iSplitR. 1: done.
-      rewrite /iSVT.
-      admit.
-    - simpl...
-      iSpecialize ("maybe_auth" $! eq_refl).
-      (* still should only be doing this if 0<n. *)
-      destruct bq' eqn:case_bq'.
-      + simpl...
-        admit.
-      + simpl...
-        admit.
-    - simpl... iExists _. iSplitR. 1: done.
-      subst.
-      admit.
-    - rewrite pweq //... iExists _. iSplitR. 1: done.
-      rewrite /iSVT. destruct (0 <? S n)%nat => //. iFrame.
-      replace (S n -1)%nat with n by lia. iFrame.
-      iExists TOKEN.
-      iSpecialize ("maybe_auth" $! eq_refl).
-      iFrame. done.
-  Admitted.
 
   (* Iterate online SVT over a list of queries. *)
   Definition SVT : val :=
     λ:"num" "den" "T" "N" "db" "qs",
-      let: "f" := SVT_AT_NF_NC_online "num" "den" "T" "N" in
+      let: "f" := oSVT "num" "den" "T" "N" in
       (rec: "SVT" "i" "bs" :=
          if: "i" = "N" then "bs" else
            match: list_nth "i" "qs" with
@@ -852,26 +292,20 @@ Section svt.
            end) #0 list_nil.
 
   (* pointwise diff priv *)
-  Lemma SVT_diffpriv (num den T : Z) (N : nat)
-    `(dDB : Distance DB) (db db' : DB) (adj : dDB db db' <= 1)
-    (qs : list val) (QS : val) (is_qs : is_list qs QS)
-    K
-    :
-    let ε := IZR num / IZR den in
-    ∀ (εpos : 0 < ε),
-      ([∗ list] q ∈ qs, wp_sensitive (Val q) 1 dDB dZ) -∗
-      ↯m ε -∗
-      ∀ RES,
-        ⤇ fill K (SVT #num #den #T #(S N)) (inject db') QS -∗
-        WP SVT #num #den #T #(S N) (inject db) QS
-          {{ v, ∃ v' : val, ⤇ fill K v' ∗ ⌜v = RES → v' = RES⌝ }}.
-  Proof with (tp_pures ; wp_pures).
+  (* Lemma SVT_diffpriv (num den T : Z) (N : nat)
+       `(dDB : Distance DB) (db db' : DB) (adj : dDB db db' <= 1)
+       (qs : list val) (QS : val) (is_qs : is_list qs QS)
+       K
+       :
+       let ε := IZR num / IZR den in
+       ∀ (εpos : 0 < ε),
+         ([∗ list] q ∈ qs, wp_sensitive (Val q) 1 dDB dZ) -∗
+         ↯m ε -∗
+         ⤇ fill K (SVT #num #den #T #(S N)) (inject db') QS -∗
+         WP SVT #num #den #T #(S N) (inject db) QS
+           {{ v, ⤇ fill K v }}.
+     Proof with (tp_pures ; wp_pures).
 
-  Abort.
-
-  (* In Justin's thesis, the discussion of choice couplings (p.70) and especially of randomized
-  privacy cost (p.71) is relevant ; it suggests that the point-wise equality proof may not be
-  required for SVT. How exactly do choice couplings help? *)
-
+     Abort. *)
 
 End svt.
